@prefix skos: <http://www.w3.org/2004/02/skos/core#> .
@prefix dcterms: <http://purl.org/dc/terms/> .
@prefix era: <http://data.europa.eu/949/> .
@prefix eralex: <http://data.europa.eu/eralex/> .
@prefix era-sh: <http://data.europa.eu/949/shapes/> .
@prefix era-sh-pava: <http://data.europa.eu/949/shapes/PAVA/> .
@prefix era-va-authcase: <http://data.europa.eu/949/concepts/va-authcases/> .


# ConceptScheme for Annex I of 2018/545
eralex:AnnexIConceptScheme a skos:ConceptScheme ;
    skos:prefLabel "Annex I Content of the Application (2018/545)"@en ;
    dcterms:source <https://eur-lex.europa.eu/legal-content/EN/TXT/?uri=CELEX%3A02018R0545-20200616#anx_I> ;
    skos:note "Each concept represents a required item from Annex I. Hierarchy is flat, as per the regulation."@en ;
    skos:hasTopConcept eralex:PAVA-AnnexI-1, eralex:PAVA-AnnexI-2, eralex:PAVA-AnnexI-3, eralex:PAVA-AnnexI-4, eralex:PAVA-AnnexI-5, eralex:PAVA-AnnexI-6, eralex:PAVA-AnnexI-7, eralex:PAVA-AnnexI-8, eralex:PAVA-AnnexI-9, eralex:PAVA-AnnexI-10, eralex:PAVA-AnnexI-11, eralex:PAVA-AnnexI-12, eralex:PAVA-AnnexI-13, eralex:PAVA-AnnexI-16, eralex:PAVA-AnnexI-17, eralex:PAVA-AnnexI-18 .

# 1. Type of application
eralex:PAVA-AnnexI-1 a skos:Concept ;
    skos:inScheme eralex:AnnexIConceptScheme ;
    skos:prefLabel "(I) 1. Type of application"@en ;
    skos:definition "Type of application (type authorisation or authorisation for placing on the market, including variants/versions, single vehicle or series)."@en ;
    skos:narrower eralex:PAVA-AnnexI-1-1, eralex:PAVA-AnnexI-1-2 ;
    dcterms:source <https://eur-lex.europa.eu/legal-content/EN/TXT/?uri=CELEX%3A02018R0545-20200616#anx_I> .

# 1.1. Type authorisation
eralex:PAVA-AnnexI-1-1 a skos:Concept ;
    skos:inScheme eralex:AnnexIConceptScheme ;
    skos:prefLabel "(I) 1.1. Type authorisation"@en ;
    skos:definition "Type authorisation (including variants and versions if any)."@en ;
    skos:broader eralex:PAVA-AnnexI-1 ;
    dcterms:source <https://eur-lex.europa.eu/legal-content/EN/TXT/?uri=CELEX%3A02018R0545-20200616#anx_I> .

# 1.2. Authorisation for placing on the market
eralex:PAVA-AnnexI-1-2 a skos:Concept ;
    skos:inScheme eralex:AnnexIConceptScheme ;
    skos:prefLabel "(I) 1.2. Authorisation for placing on the market"@en ;
    skos:definition "Authorisation for placing on the market (single vehicle or series of vehicles)."@en ;
    skos:broader eralex:PAVA-AnnexI-1 ;
    dcterms:source <https://eur-lex.europa.eu/legal-content/EN/TXT/?uri=CELEX%3A02018R0545-20200616#anx_I> .

# 2. Authorisation case
eralex:PAVA-AnnexI-2 a skos:Concept ;
    skos:inScheme eralex:AnnexIConceptScheme ;
    skos:prefLabel "(I) 2. Authorisation case"@en ;
    skos:definition "Authorisation case (first, new, extended area of use, renewed, conformity to type)."@en ;
    skos:narrower eralex:PAVA-AnnexI-2-1, eralex:PAVA-AnnexI-2-2, eralex:PAVA-AnnexI-2-3, eralex:PAVA-AnnexI-2-4, eralex:PAVA-AnnexI-2-5 ;
    dcterms:source <https://eur-lex.europa.eu/legal-content/EN/TXT/?uri=CELEX%3A02018R0545-20200616#anx_I> .

# 2.1. First authorisation
eralex:PAVA-AnnexI-2-1 a skos:Concept ;
    skos:inScheme eralex:AnnexIConceptScheme ;
    skos:prefLabel "(I) 2.1. First authorisation"@en ;
    skos:definition "First authorisation."@en ;
    skos:broader eralex:PAVA-AnnexI-2 ;
    dcterms:source <https://eur-lex.europa.eu/legal-content/EN/TXT/?uri=CELEX%3A02018R0545-20200616#anx_I> .

# 2.2. New authorisation
eralex:PAVA-AnnexI-2-2 a skos:Concept ;
    skos:inScheme eralex:AnnexIConceptScheme ;
    skos:prefLabel "(I) 2.2. New authorisation"@en ;
    skos:definition "New authorisation."@en ;
    skos:broader eralex:PAVA-AnnexI-2 ;
    dcterms:source <https://eur-lex.europa.eu/legal-content/EN/TXT/?uri=CELEX%3A02018R0545-20200616#anx_I> .

# 2.3. Extended area of use
eralex:PAVA-AnnexI-2-3 a skos:Concept ;
    skos:inScheme eralex:AnnexIConceptScheme ;
    skos:prefLabel "(I) 2.3. Extended area of use"@en ;
    skos:definition "Extended area of use."@en ;
    skos:broader eralex:PAVA-AnnexI-2 ;
    dcterms:source <https://eur-lex.europa.eu/legal-content/EN/TXT/?uri=CELEX%3A02018R0545-20200616#anx_I> .

# 2.4. Renewed type authorisation
eralex:PAVA-AnnexI-2-4 a skos:Concept ;
    skos:inScheme eralex:AnnexIConceptScheme ;
    skos:prefLabel "(I) 2.4. Renewed type authorisation"@en ;
    skos:definition "Renewed type authorisation."@en ;
    skos:broader eralex:PAVA-AnnexI-2 ;
    dcterms:source <https://eur-lex.europa.eu/legal-content/EN/TXT/?uri=CELEX%3A02018R0545-20200616#anx_I> .

# 2.5. Authorisation in conformity to type
eralex:PAVA-AnnexI-2-5 a skos:Concept ;
    skos:inScheme eralex:AnnexIConceptScheme ;
    skos:prefLabel "(I) 2.5. Authorisation in conformity to type"@en ;
    skos:definition "Authorisation in conformity to type."@en ;
    skos:broader eralex:PAVA-AnnexI-2 ;
    dcterms:source <https://eur-lex.europa.eu/legal-content/EN/TXT/?uri=CELEX%3A02018R0545-20200616#anx_I> .

# 3. Area of use
eralex:PAVA-AnnexI-3 a skos:Concept ;
    skos:inScheme eralex:AnnexIConceptScheme ;
    skos:prefLabel "(I) 3. Area of use"@en ;
    skos:definition "Area of use (Member States, networks, border stations, extended area, whole EU network)."@en ;
    skos:narrower eralex:PAVA-AnnexI-3-1, eralex:PAVA-AnnexI-3-2, eralex:PAVA-AnnexI-3-3, eralex:PAVA-AnnexI-3-4, eralex:PAVA-AnnexI-3-5 ;
    dcterms:source <https://eur-lex.europa.eu/legal-content/EN/TXT/?uri=CELEX%3A02018R0545-20200616#anx_I> .

# 3.1. Member States
eralex:PAVA-AnnexI-3-1 a skos:Concept ;
    skos:inScheme eralex:AnnexIConceptScheme ;
    skos:prefLabel "(I) 3.1. Member States"@en ;
    skos:definition "Member States."@en ;
    skos:broader eralex:PAVA-AnnexI-3 ;
    dcterms:source <https://eur-lex.europa.eu/legal-content/EN/TXT/?uri=CELEX%3A02018R0545-20200616#anx_I> .

# 3.2. Networks (per Member State)
eralex:PAVA-AnnexI-3-2 a skos:Concept ;
    skos:inScheme eralex:AnnexIConceptScheme ;
    skos:prefLabel "(I) 3.2. Networks (per Member State)"@en ;
    skos:definition "Networks (per Member State)."@en ;
    skos:broader eralex:PAVA-AnnexI-3 ;
    dcterms:source <https://eur-lex.europa.eu/legal-content/EN/TXT/?uri=CELEX%3A02018R0545-20200616#anx_I> .

# 3.3. Border stations
eralex:PAVA-AnnexI-3-3 a skos:Concept ;
    skos:inScheme eralex:AnnexIConceptScheme ;
    skos:prefLabel "(I) 3.3. Border stations"@en ;
    skos:definition "Stations with similar network characteristics in neighbouring Member States when those stations are close to the border."@en ;
    skos:broader eralex:PAVA-AnnexI-3 ;
    dcterms:source <https://eur-lex.europa.eu/legal-content/EN/TXT/?uri=CELEX%3A02018R0545-20200616#anx_I> .

# 3.4. Extended area of use
eralex:PAVA-AnnexI-3-4 a skos:Concept ;
    skos:inScheme eralex:AnnexIConceptScheme ;
    skos:prefLabel "(I) 3.4. Extended area of use"@en ;
    skos:definition "Definition of the extended area of use (only applicable for the authorisation case ‘Extended area of use’)."@en ;
    skos:broader eralex:PAVA-AnnexI-3 ;
    dcterms:source <https://eur-lex.europa.eu/legal-content/EN/TXT/?uri=CELEX%3A02018R0545-20200616#anx_I> .

# 3.5. Whole EU network
eralex:PAVA-AnnexI-3-5 a skos:Concept ;
    skos:inScheme eralex:AnnexIConceptScheme ;
    skos:prefLabel "(I) 3.5. Whole EU network"@en ;
    skos:definition "Whole EU network (applicable for wagons conforming with chapter 7.1.2 of TSI WAG)."@en ;
    skos:broader eralex:PAVA-AnnexI-3 ;
    dcterms:source <https://eur-lex.europa.eu/legal-content/EN/TXT/?uri=CELEX%3A02018R0545-20200616#anx_I> .

# 4. Issuing authority
eralex:PAVA-AnnexI-4 a skos:Concept ;
    skos:inScheme eralex:AnnexIConceptScheme ;
    skos:prefLabel "(I) 4. Issuing authority"@en ;
    skos:definition "Issuing authority (Agency or national safety authority, as applicable)."@en ;
    skos:narrower eralex:PAVA-AnnexI-4-1, eralex:PAVA-AnnexI-4-2 ;
    dcterms:source <https://eur-lex.europa.eu/legal-content/EN/TXT/?uri=CELEX%3A02018R0545-20200616#anx_I> .

# 4.1. The Agency
eralex:PAVA-AnnexI-4-1 a skos:Concept ;
    skos:inScheme eralex:AnnexIConceptScheme ;
    skos:prefLabel "(I) 4.1. The Agency"@en ;
    skos:definition "The Agency: area of use covers networks in 1 or more Member States."@en ;
    skos:broader eralex:PAVA-AnnexI-4 ;
    dcterms:source <https://eur-lex.europa.eu/legal-content/EN/TXT/?uri=CELEX%3A02018R0545-20200616#anx_I> .

# 4.2. National safety authority
eralex:PAVA-AnnexI-4-2 a skos:Concept ;
    skos:inScheme eralex:AnnexIConceptScheme ;
    skos:prefLabel "(I) 4.2. National safety authority"@en ;
    skos:definition "The national safety authority of the Member State concerned: area of use covering 1 Member State."@en ;
    skos:broader eralex:PAVA-AnnexI-4 ;
    dcterms:source <https://eur-lex.europa.eu/legal-content/EN/TXT/?uri=CELEX%3A02018R0545-20200616#anx_I> .

# 5. Applicant's information
eralex:PAVA-AnnexI-5 a skos:Concept ;
    skos:inScheme eralex:AnnexIConceptScheme ;
    skos:prefLabel "(I) 5. Applicant's information"@en ;
    skos:definition "Applicant's information (name, address, contact details, VAT, etc.)."@en ;
    dcterms:source <https://eur-lex.europa.eu/legal-content/EN/TXT/?uri=CELEX%3A02018R0545-20200616#anx_I> .

# 6. Contact person information
eralex:PAVA-AnnexI-6 a skos:Concept ;
    skos:inScheme eralex:AnnexIConceptScheme ;
    skos:prefLabel "(I) 6. Contact person information"@en ;
    skos:definition "Contact person information (name, function, address, phone, email, languages)."@en ;
    dcterms:source <https://eur-lex.europa.eu/legal-content/EN/TXT/?uri=CELEX%3A02018R0545-20200616#anx_I> .

# 7. Current vehicle type authorisation holder
eralex:PAVA-AnnexI-7 a skos:Concept ;
    skos:inScheme eralex:AnnexIConceptScheme ;
    skos:prefLabel "(I) 7. Current vehicle type authorisation holder"@en ;
    skos:definition "Current vehicle type authorisation holder (if not first authorisation)."@en ;
    dcterms:source <https://eur-lex.europa.eu/legal-content/EN/TXT/?uri=CELEX%3A02018R0545-20200616#anx_I> .

# 8. Assessment bodies information
eralex:PAVA-AnnexI-8 a skos:Concept ;
    skos:inScheme eralex:AnnexIConceptScheme ;
    skos:prefLabel "(I) 8. Assessment bodies information"@en ;
    skos:definition "Assessment bodies information (notified bodies, designated bodies, CSM RA assessment body)."@en ;
    dcterms:source <https://eur-lex.europa.eu/legal-content/EN/TXT/?uri=CELEX%3A02018R0545-20200616#anx_I> .

# 9. Pre-engagement
eralex:PAVA-AnnexI-9 a skos:Concept ;
    skos:inScheme eralex:AnnexIConceptScheme ;
    skos:prefLabel "(I) 9. Pre-engagement"@en ;
    skos:definition "Pre-engagement (reference to pre-engagement baseline, other project info)."@en ;
    skos:narrower eralex:PAVA-AnnexI-9-1, eralex:PAVA-AnnexI-9-2 ;
    dcterms:source <https://eur-lex.europa.eu/legal-content/EN/TXT/?uri=CELEX%3A02018R0545-20200616#anx_I> .

# 9.1. Reference to pre-engagement baseline
eralex:PAVA-AnnexI-9-1 a skos:Concept ;
    skos:inScheme eralex:AnnexIConceptScheme ;
    skos:prefLabel "(I) 9.1. Reference to pre-engagement baseline"@en ;
    skos:definition "Reference to pre-engagement baseline."@en ;
    skos:broader eralex:PAVA-AnnexI-9 ;
    dcterms:source <https://eur-lex.europa.eu/legal-content/EN/TXT/?uri=CELEX%3A02018R0545-20200616#anx_I> .

# 9.2. Other project information
eralex:PAVA-AnnexI-9-2 a skos:Concept ;
    skos:inScheme eralex:AnnexIConceptScheme ;
    skos:prefLabel "(I) 9.2. Other project information"@en ;
    skos:definition "Other project information relevant to pre-engagement."@en ;
    skos:broader eralex:PAVA-AnnexI-9 ;
    dcterms:source <https://eur-lex.europa.eu/legal-content/EN/TXT/?uri=CELEX%3A02018R0545-20200616#anx_I> .

# 10. Description of the vehicle type
eralex:PAVA-AnnexI-10 a skos:Concept ;
    skos:inScheme eralex:AnnexIConceptScheme ;
    skos:prefLabel "(I) 10. Description of the vehicle type"@en ;
    skos:definition "Description of the vehicle type (type ID, versions, variants, date of record, name, category, subcategory)."@en ;
    skos:narrower eralex:PAVA-AnnexI-10-1, eralex:PAVA-AnnexI-10-2 ;
    dcterms:source <https://eur-lex.europa.eu/legal-content/EN/TXT/?uri=CELEX%3A02018R0545-20200616#anx_I> .

# 10.1. Type identification
eralex:PAVA-AnnexI-10-1 a skos:Concept ;
    skos:inScheme eralex:AnnexIConceptScheme ;
    skos:prefLabel "(I) 10.1. Type identification"@en ;
    skos:definition "Type identification (ID, name, date of record)."@en ;
    skos:broader eralex:PAVA-AnnexI-10 ;
    dcterms:source <https://eur-lex.europa.eu/legal-content/EN/TXT/?uri=CELEX%3A02018R0545-20200616#anx_I> .

# 10.2. Vehicle type versions (when applicable)
eralex:PAVA-AnnexI-10-2 a skos:Concept ;
    skos:inScheme eralex:AnnexIConceptScheme ;
    skos:prefLabel "(I) 10.2. Vehicle type versions (when applicable)"@en ;
    skos:definition "Vehicle type versions as defined in Decision 2011/665/EU Annex II, when applicable."@en ;
    skos:broader eralex:PAVA-AnnexI-10 ;
    dcterms:source <https://eur-lex.europa.eu/legal-content/EN/TXT/?uri=CELEX%3A02018R0545-20200616#anx_I> .

# 10.3. Vehicle type variants (when applicable)
eralex:PAVA-AnnexI-10-3 a skos:Concept ;
    skos:inScheme eralex:AnnexIConceptScheme ;
    skos:prefLabel "(I) 10.3. Vehicle type variants (when applicable)"@en ;
    skos:definition "Vehicle type variants as defined in Decision 2011/665/EU Annex II, when applicable."@en ;
    skos:broader eralex:PAVA-AnnexI-10 ;
    dcterms:source <https://eur-lex.europa.eu/legal-content/EN/TXT/?uri=CELEX%3A02018R0545-20200616#anx_I> .

# 10.4. Date of record in ERATV (not applicable for first authorisation)
eralex:PAVA-AnnexI-10-4 a skos:Concept ;
    skos:inScheme eralex:AnnexIConceptScheme ;
    skos:prefLabel "(I) 10.4. Date of record in ERATV (not applicable for first authorisation)"@en ;
    skos:definition "Date of record in the European Register of Authorised Types of Vehicles (ERATV), not applicable for first authorisation."@en ;
    skos:broader eralex:PAVA-AnnexI-10 ;
    dcterms:source <https://eur-lex.europa.eu/legal-content/EN/TXT/?uri=CELEX%3A02018R0545-20200616#anx_I> .

# 10.5. Type name (*)
eralex:PAVA-AnnexI-10-5 a skos:Concept ;
    skos:inScheme eralex:AnnexIConceptScheme ;
    skos:prefLabel "(I) 10.5. Type name (*)"@en ;
    skos:definition "Type name as specified in Decision 2011/665/EU Annex II."@en ;
    skos:broader eralex:PAVA-AnnexI-10 ;
    dcterms:source <https://eur-lex.europa.eu/legal-content/EN/TXT/?uri=CELEX%3A02018R0545-20200616#anx_I> .

# 10.6. Alternative type name (when applicable)
eralex:PAVA-AnnexI-10-6 a skos:Concept ;
    skos:inScheme eralex:AnnexIConceptScheme ;
    skos:prefLabel "(I) 10.6. Alternative type name (when applicable)"@en ;
    skos:definition "Alternative type name, when applicable, as specified in Decision 2011/665/EU Annex II."@en ;
    skos:broader eralex:PAVA-AnnexI-10 ;
    dcterms:source <https://eur-lex.europa.eu/legal-content/EN/TXT/?uri=CELEX%3A02018R0545-20200616#anx_I> .

# 10.7. Category (*)
eralex:PAVA-AnnexI-10-7 a skos:Concept ;
    skos:inScheme eralex:AnnexIConceptScheme ;
    skos:prefLabel "(I) 10.7. Category (*)"@en ;
    skos:definition "Category of the vehicle type as specified in Decision 2011/665/EU Annex II."@en ;
    skos:broader eralex:PAVA-AnnexI-10 ;
    dcterms:source <https://eur-lex.europa.eu/legal-content/EN/TXT/?uri=CELEX%3A02018R0545-20200616#anx_I> .

# 10.8. Subcategory (*)
eralex:PAVA-AnnexI-10-8 a skos:Concept ;
    skos:inScheme eralex:AnnexIConceptScheme ;
    skos:prefLabel "(I) 10.8. Subcategory (*)"@en ;
    skos:definition "Subcategory of the vehicle type as specified in Decision 2011/665/EU Annex II."@en ;
    skos:broader eralex:PAVA-AnnexI-10 ;
    dcterms:source <https://eur-lex.europa.eu/legal-content/EN/TXT/?uri=CELEX%3A02018R0545-20200616#anx_I> .

# 11. Information on the vehicles
eralex:PAVA-AnnexI-11 a skos:Concept ;
    skos:inScheme eralex:AnnexIConceptScheme ;
    skos:prefLabel "(I) 11. Information on the vehicles"@en ;
    skos:definition "Information on the vehicles (EVN numbers, pre-reserved numbers, other identification)."@en ;
    skos:narrower eralex:PAVA-AnnexI-11-1, eralex:PAVA-AnnexI-11-2 ;
    dcterms:source <https://eur-lex.europa.eu/legal-content/EN/TXT/?uri=CELEX%3A02018R0545-20200616#anx_I> .

# 11.1. EVN numbers
eralex:PAVA-AnnexI-11-1 a skos:Concept ;
    skos:inScheme eralex:AnnexIConceptScheme ;
    skos:prefLabel "(I) 11.1. EVN numbers"@en ;
    skos:definition "European Vehicle Numbers (EVN) assigned to the vehicles."@en ;
    skos:broader eralex:PAVA-AnnexI-11 ;
    dcterms:source <https://eur-lex.europa.eu/legal-content/EN/TXT/?uri=CELEX%3A02018R0545-20200616#anx_I> .

# 11.2. Other identification
eralex:PAVA-AnnexI-11-2 a skos:Concept ;
    skos:inScheme eralex:AnnexIConceptScheme ;
    skos:prefLabel "(I) 11.2. Other identification"@en ;
    skos:definition "Other identification (pre-reserved numbers, etc.)."@en ;
    skos:broader eralex:PAVA-AnnexI-11 ;
    dcterms:source <https://eur-lex.europa.eu/legal-content/EN/TXT/?uri=CELEX%3A02018R0545-20200616#anx_I> .

# 12. Reference to existing vehicle type authorisation (not applicable in case of first authorisation) (M)
eralex:PAVA-AnnexI-12 a skos:Concept ;
    skos:inScheme eralex:AnnexIConceptScheme ;
    skos:prefLabel "(I) 12. Reference to existing vehicle type authorisation (not applicable in case of first authorisation)"@en ;
    skos:definition "Reference to existing vehicle type authorisation, not applicable for first authorisation."@en ;
    skos:related era-va-authcase:RENEW, era-va-authcase:EXT, era-va-authcase:NEW, era-va-authcase:C2T ;
    dcterms:source <https://eur-lex.europa.eu/legal-content/EN/TXT/?uri=CELEX%3A02018R0545-20200616#anx_I> .

# 13. Description of the changes as compared to the authorised vehicle type (only applicable in case of a new authorisation) (M)
eralex:PAVA-AnnexI-13 a skos:Concept ;
    skos:inScheme eralex:AnnexIConceptScheme ;
    skos:prefLabel "(I) 13. Description of the changes as compared to the authorised vehicle type (only applicable in case of a new authorisation)"@en ;
    skos:definition "Description of the changes as compared to the authorised vehicle type (only applicable in case of a new authorisation)."@en ;
    skos:related eralex:PAVA-AnnexI-2-2, era-va-authcase:NEW ;
    dcterms:source <https://eur-lex.europa.eu/legal-content/EN/TXT/?uri=CELEX%3A02018R0545-20200616#anx_I> .

# 16. Applicable rules (M)
eralex:PAVA-AnnexI-16 a skos:Concept ;
    skos:inScheme eralex:AnnexIConceptScheme ;
    skos:prefLabel "(I) 16. Applicable rules (M)"@en ;
    skos:definition "Applicable rules (TSIs, national rules, non-applications, updated rules, etc.)."@en ;
    skos:narrower eralex:PAVA-AnnexI-16-1, eralex:PAVA-AnnexI-16-2, eralex:PAVA-AnnexI-16-3, eralex:PAVA-AnnexI-16-4, eralex:PAVA-AnnexI-16-5, eralex:PAVA-AnnexI-16-6, eralex:PAVA-AnnexI-16-7 ;
    dcterms:source <https://eur-lex.europa.eu/legal-content/EN/TXT/?uri=CELEX%3A02018R0545-20200616#anx_I> .

# 16.1. TSIs
eralex:PAVA-AnnexI-16-1 a skos:Concept ;
    skos:inScheme eralex:AnnexIConceptScheme ;
    skos:prefLabel "(I) 16.1. TSIs"@en ;
    skos:definition "Technical Specifications for Interoperability (TSIs), including the legal reference in the Official Journal of the European Union."@en ;
    skos:broader eralex:PAVA-AnnexI-16 ;
    dcterms:source <https://eur-lex.europa.eu/legal-content/EN/TXT/?uri=CELEX%3A02018R0545-20200616#anx_I> .

# 16.2. Specific TSIs clauses for an area of use covering the whole EU network (when applicable)
eralex:PAVA-AnnexI-16-2 a skos:Concept ;
    skos:inScheme eralex:AnnexIConceptScheme ;
    skos:prefLabel "(I) 16.2. Specific TSIs clauses for an area of use covering the whole EU network (when applicable)"@en ;
    skos:definition "Specific TSIs clauses for an area of use covering the whole EU network, when applicable."@en ;
    skos:broader eralex:PAVA-AnnexI-16 ;
    dcterms:source <https://eur-lex.europa.eu/legal-content/EN/TXT/?uri=CELEX%3A02018R0545-20200616#anx_I> .

# 16.3. Specification of the selection of requirements from a newer version of a TSI as compared to the TSI applicable for the assessment (including withdrawn requirements) (when applicable)
eralex:PAVA-AnnexI-16-3 a skos:Concept ;
    skos:inScheme eralex:AnnexIConceptScheme ;
    skos:prefLabel "(I) 16.3. Specification of the selection of requirements from a newer version of a TSI as compared to the TSI applicable for the assessment (including withdrawn requirements) (when applicable)"@en ;
    skos:definition "Specification of the selection of requirements from a newer version of a TSI as compared to the TSI applicable for the assessment, including withdrawn requirements, when applicable."@en ;
    skos:broader eralex:PAVA-AnnexI-16 ;
    dcterms:source <https://eur-lex.europa.eu/legal-content/EN/TXT/?uri=CELEX%3A02018R0545-20200616#anx_I> .

# 16.4. National rules (when applicable)
eralex:PAVA-AnnexI-16-4 a skos:Concept ;
    skos:inScheme eralex:AnnexIConceptScheme ;
    skos:prefLabel "(I) 16.4. National rules (when applicable)"@en ;
    skos:definition "National rules, when applicable."@en ;
    skos:broader eralex:PAVA-AnnexI-16 ;
    dcterms:source <https://eur-lex.europa.eu/legal-content/EN/TXT/?uri=CELEX%3A02018R0545-20200616#anx_I> .

# 16.5. Non-applications of TSIs according to the provisions of Article 7 of Directive (EU) 2016/797 (when applicable)
eralex:PAVA-AnnexI-16-5 a skos:Concept ;
    skos:inScheme eralex:AnnexIConceptScheme ;
    skos:prefLabel "(I) 16.5. Non-applications of TSIs according to the provisions of Article 7 of Directive (EU) 2016/797 (when applicable)"@en ;
    skos:definition "Non-applications of TSIs according to the provisions of Article 7 of Directive (EU) 2016/797, when applicable."@en ;
    skos:broader eralex:PAVA-AnnexI-16 ;
    dcterms:source <https://eur-lex.europa.eu/legal-content/EN/TXT/?uri=CELEX%3A02018R0545-20200616#anx_I> .

# 16.6. Applicable rules for the extended area of use
eralex:PAVA-AnnexI-16-6 a skos:Concept ;
    skos:inScheme eralex:AnnexIConceptScheme ;
    skos:prefLabel "(I) 16.6. Applicable rules for the extended area of use"@en ;
    skos:definition "Applicable rules for the extended area of use."@en ;
    skos:broader eralex:PAVA-AnnexI-16 ;
    dcterms:source <https://eur-lex.europa.eu/legal-content/EN/TXT/?uri=CELEX%3A02018R0545-20200616#anx_I> .

# 16.7. Updated TSIs and/or national rules (only applicable for renewed type authorisation)
eralex:PAVA-AnnexI-16-7 a skos:Concept ;
    skos:inScheme eralex:AnnexIConceptScheme ;
    skos:prefLabel "(I) 16.7. Updated TSIs and/or national rules (only applicable for renewed type authorisation)"@en ;
    skos:definition "Updated TSIs and/or national rules, only applicable for renewed type authorisation."@en ;
    skos:broader eralex:PAVA-AnnexI-16 ;
    dcterms:source <https://eur-lex.europa.eu/legal-content/EN/TXT/?uri=CELEX%3A02018R0545-20200616#anx_I> .

# 17. Applicant's confirmation and signature
eralex:PAVA-AnnexI-17 a skos:Concept ;
    skos:inScheme eralex:AnnexIConceptScheme ;
    skos:prefLabel "(I) 17. Applicant's confirmation and signature"@en ;
    skos:definition "Applicant's confirmation and signature."@en ;
    dcterms:source <https://eur-lex.europa.eu/legal-content/EN/TXT/?uri=CELEX%3A02018R0545-20200616#anx_I> .

# 18. Annexes
eralex:PAVA-AnnexI-18 a skos:Concept ;
    skos:inScheme eralex:AnnexIConceptScheme ;
    skos:prefLabel "(I) 18. Annexes"@en ;
    skos:definition "Annexes (supporting evidence, mapping tables, declarations, technical files, etc.)."@en ;
    dcterms:source <https://eur-lex.europa.eu/legal-content/EN/TXT/?uri=CELEX%3A02018R0545-20200616#anx_I> .