@base <http://data.europa.eu/949/> .
@prefix era: <http://data.europa.eu/949/> .
@prefix era-sh: <http://data.europa.eu/949/shapes/> .

# From examples
@prefix erapod: <https://storage.inrupt.com/ea779a2c-b43d-4723-8b1a-aaa8990dd576/data/eradis/> .
@prefix gotham: <https://batman.fandom.com/wiki/> .

# General
@prefix as:    <https://www.w3.org/ns/activitystreams#> .
@prefix cc:    <http://creativecommons.org/ns#> .
@prefix dash:  <http://datashapes.org/dash#> .
@prefix dcat:  <http://www.w3.org/ns/dcat#> .
@prefix dcterms: <http://purl.org/dc/terms/> .
@prefix dct:  <http://purl.org/dc/terms/> .
@prefix dul:  <http://www.ontologydesignpatterns.org/ont/dul/DUL.owl#> .
@prefix foaf: <http://xmlns.com/foaf/0.1/> .
@prefix geo:  <http://www.opengis.net/ont/geosparql#> .
@prefix gr:   <http://purl.org/goodrelations/v1#> .
@prefix org:  <http://www.w3.org/ns/org#> .
@prefix owl:  <http://www.w3.org/2002/07/owl#> .
@prefix prov: <http://www.w3.org/ns/prov#> .
@prefix rdfs: <http://www.w3.org/2000/01/rdf-schema#> .
@prefix rdf:  <http://www.w3.org/1999/02/22-rdf-syntax-ns#> .
@prefix schema:  <http://schema.org/> .
@prefix sh:   <http://www.w3.org/ns/shacl#> .
@prefix skos: <http://www.w3.org/2004/02/skos/core#> .
@prefix time: <http://www.w3.org/2006/time#> .
@prefix unit: <http://qudt.org/vocab/unit/> .
@prefix vcard: <http://www.w3.org/2006/vcard/ns#> .
@prefix vpa: <http://w3id.org/vpa#> .
@prefix vs: <http://www.w3.org/2003/06/sw-vocab-status/ns#> .
@prefix xsd: <http://www.w3.org/2001/XMLSchema#> .

# Domain-specific
@prefix era-cld: <http://data.europa.eu/949/eradis/clds/> .
@prefix era-cfg: <http://data.europa.eu/949/vehicleTypeConfigurations/> .
@prefix era-ecd: <http://data.europa.eu/949/eradis/declarations/> .
@prefix eralex: <http://data.europa.eu/949/requirements/> .
@prefix rorg: <http://data.europa.eu/949/organisations/> .
@prefix lorg: <http://data.europa.eu/949/organisations/sites/> .
@prefix uorg: <http://data.europa.eu/949/organisations/units/> .
@prefix eratv: <http://data.europa.eu/949/vehicleTypes/> .
@prefix erava: <http://data.europa.eu/949/vehicleTypeAuthorisations/> .
@prefix eravr: <http://data.europa.eu/949/vehicles/registrations/> .
@prefix evr: <http://data.europa.eu/949/vehicles/> .
@prefix iss: <http://data.europa.eu/949/iss/> . 


# Relevant SKOS Concept Schemes
@prefix era-skos: <http://data.europa.eu/949/concepts/> .
@prefix era-cld-types: <http://data.europa.eu/949/concepts/cld-types/> .
@prefix era-ecd-types: <http://data.europa.eu/949/concepts/ecd-types/> .
@prefix era-cld-modules: <http://data.europa.eu/949/concepts/cld-modules/> .
@prefix era-organisation-roles: <http://data.europa.eu/949/concepts/organisation-roles/> .
@prefix era-states: <http://data.europa.eu/949/concepts/states/> .
@prefix era-va-authcase: <http://data.europa.eu/949/concepts/va-authcases/> .
@prefix era-vtc: <http://data.europa.eu/949/concepts/vehicle-type-configurations/> .
@prefix era-vehicle-types-eratv: <http://data.europa.eu/949/concepts/vehicle-types/eratv/> .
# unused @prefix era-vehicle-types: <http://data.europa.eu/949/concepts/vehicle-types/> .
@prefix era-ntg-rinf: <http://data.europa.eu/949/concepts/nominal-track-gauges/rinf/> .
@prefix era-ess-rinf: <http://data.europa.eu/949/concepts/energy-supply-systems/rinf/> .
@prefix era-noic: <http://data.europa.eu/949/concepts/noise-categories/NoiseCategories/> .
@prefix era-va-trm: <http://data.europa.eu/949/concepts/va-type-registration-methods/> .

 # WARNING: DO NOT (YET) EXIST
@prefix era-permission-types: <http://data.europa.eu/949/concepts/permission-types/> .
@prefix era-ecm-maintenance-functions: <http://data.europa.eu/949/concepts/ecm-maintenance-functions/> .
@prefix era-lex-sections: <http://data.europa.eu/949/concepts/requirements/section/> .
@prefix era-pava-at: <http://data.europa.eu/949/concepts/va-authassessment-types/> .
@prefix era-etcsmanspecset: <http://data.europa.eu/949/concepts/etcs-mandatory-specifications-set/> .
@prefix erava-orgroletasks: <http://data.europa.eu/949/concepts/org-role-tasks/> .
@prefix issform:  <http://era.europa.eu/forms/iss/> . 

# From ISS
@prefix iss-skos: <https://raw.githubusercontent.com/Interoperable-data/ISS_vocabulary/refs/heads/main/iss-skos/> .
@prefix iss-rs:   <http://data.europa.eu/949/iss/concepts/record-statuses/> .
@prefix iss-dcs: <http://data.europa.eu/949/iss/concepts/document-statuses/> .

# EU Countries
@prefix vac: <https://raw.githubusercontent.com/Interoperable-data/automate-va/refs/heads/dev-lws/TTL/> .

# Properties to be post-processed, if shacl-form 
@prefix update: <http://data.europa.eu/949/update/> .

# ConceptScheme for Annex I of 2018/545
eralex:AnnexIConceptScheme a skos:ConceptScheme ;
    skos:prefLabel "Annex I Content of the Application (2018/545)"@en ;
    dcterms:source <https://eur-lex.europa.eu/legal-content/EN/TXT/?uri=CELEX%3A02018R0545-20200616#anx_I> ;
    skos:note "Each concept represents a required item from Annex I. Hierarchy is flat, as per the regulation."@en ;
    skos:hasTopConcept eralex:PAVA-AnnexI-1, eralex:PAVA-AnnexI-2, eralex:PAVA-AnnexI-3, eralex:PAVA-AnnexI-4, eralex:PAVA-AnnexI-5, eralex:PAVA-AnnexI-6, eralex:PAVA-AnnexI-7, eralex:PAVA-AnnexI-8, eralex:PAVA-AnnexI-9, eralex:PAVA-AnnexI-10, eralex:PAVA-AnnexI-11, eralex:PAVA-AnnexI-12, eralex:PAVA-AnnexI-13, eralex:PAVA-AnnexI-16, eralex:PAVA-AnnexI-17, eralex:PAVA-AnnexI-18 .

# 1. Type of application
eralex:PAVA-AnnexI-1 a skos:Concept , sh:NodeShape ;
    skos:inScheme eralex:AnnexIConceptScheme ;
    skos:prefLabel "(I) 1. Type of application"@en ;
    skos:definition "Type of application (type authorisation or authorisation for placing on the market, including variants/versions, single vehicle or series)."@en ;
    skos:narrower eralex:PAVA-AnnexI-1-1, eralex:PAVA-AnnexI-1-2 ;
    sh:targetClass era:VehicleTypeAuthorisationCase ;
    sh:xone (
        [ sh:path era:typeRegistrationMethod ; sh:minCount 1 ; sh:maxCount 1 ; sh:message "Type authorisation: typeRegistrationMethod must be present (I 1.1)."@en ; sh:severity sh:Info ]
        [ sh:path era:typeRegistrationMethod ; sh:maxCount 0 ; sh:message "Authorisation for placing on the market: typeRegistrationMethod must NOT be present (I 1.2)."@en ; sh:severity sh:Info ]
    ) ;
    dcterms:source <https://eur-lex.europa.eu/legal-content/EN/TXT/?uri=CELEX%3A02018R0545-20200616#anx_I> .

# 1.1. Type authorisation
eralex:PAVA-AnnexI-1-1 a skos:Concept ;
    skos:inScheme eralex:AnnexIConceptScheme ;
    skos:prefLabel "(I) 1.1. Type authorisation"@en ;
    skos:definition "Type authorisation (including variants and versions if any). This applies when the application is for a type authorisation, including all versions and variants."@en ;
    skos:broader eralex:PAVA-AnnexI-1 ;
    dcterms:source <https://eur-lex.europa.eu/legal-content/EN/TXT/?uri=CELEX%3A02018R0545-20200616#anx_I> .

# 1.2. Authorisation for placing on the market
eralex:PAVA-AnnexI-1-2 a skos:Concept ;
    skos:inScheme eralex:AnnexIConceptScheme ;
    skos:prefLabel "(I) 1.2. Authorisation for placing on the market"@en ;
    skos:definition "Authorisation for placing on the market (single vehicle or series of vehicles). This applies when the application is for placing vehicles on the market, not for type authorisation."@en ;
    skos:broader eralex:PAVA-AnnexI-1 ;
    dcterms:source <https://eur-lex.europa.eu/legal-content/EN/TXT/?uri=CELEX%3A02018R0545-20200616#anx_I> .

# 2. Authorisation case
eralex:PAVA-AnnexI-2 a skos:Concept , sh:NodeShape ;
    skos:inScheme eralex:AnnexIConceptScheme ;
    skos:prefLabel "(I) 2. Authorisation case"@en ;
    skos:definition "Authorisation case (first, new, extended area of use, renewed, conformity to type)."@en ;
    skos:narrower eralex:PAVA-AnnexI-2-1, eralex:PAVA-AnnexI-2-2, eralex:PAVA-AnnexI-2-3, eralex:PAVA-AnnexI-2-4, eralex:PAVA-AnnexI-2-5 ;
    sh:targetClass era:VehicleTypeAuthorisationCase ;
    sh:property [
        sh:path vpa:permissionType ;
        sh:minCount 1 ;
        sh:maxCount 1 ;
        sh:in ( era-va-authcase:FA era-va-authcase:NEW era-va-authcase:EXT era-va-authcase:RENEW era-va-authcase:C2T ) ;
        sh:xone (
            [ sh:hasValue era-va-authcase:FA ; sh:message "Authorisation case is 'First authorisation'."@en ; sh:severity sh:Info ]
            [ sh:hasValue era-va-authcase:NEW ; sh:message "Authorisation case is 'New authorisation'."@en ; sh:severity sh:Info ]
            [ sh:hasValue era-va-authcase:EXT ; sh:message "Authorisation case is 'Extended area of use'."@en ; sh:severity sh:Info ]
            [ sh:hasValue era-va-authcase:RENEW ; sh:message "Authorisation case is 'Renewed type authorisation'."@en ; sh:severity sh:Info ]
            [ sh:hasValue era-va-authcase:C2T ; sh:message "Authorisation case is 'Authorisation in conformity to type'."@en ; sh:severity sh:Info ]
        ) ;
        sh:message "Authorisation case must have exactly one vpa:permissionType linking to one of: FA, NEW, EXT, RENEW, C2T."@en ;
        sh:severity sh:Violation
    ] ;
    dcterms:source <https://eur-lex.europa.eu/legal-content/EN/TXT/?uri=CELEX%3A02018R0545-20200616#anx_I> .

# 2.1. First authorisation
eralex:PAVA-AnnexI-2-1 a skos:Concept ;
    skos:inScheme eralex:AnnexIConceptScheme ;
    skos:prefLabel "(I) 2.1. First authorisation"@en ;
    skos:definition "First authorisation."@en ;
    skos:broader eralex:PAVA-AnnexI-2 ;
    dcterms:source <https://eur-lex.europa.eu/legal-content/EN/TXT/?uri=CELEX%3A02018R0545-20200616#anx_I> .

# 2.2. New authorisation
eralex:PAVA-AnnexI-2-2 a skos:Concept ;
    skos:inScheme eralex:AnnexIConceptScheme ;
    skos:prefLabel "(I) 2.2. New authorisation"@en ;
    skos:definition "New authorisation."@en ;
    skos:broader eralex:PAVA-AnnexI-2 ;
    dcterms:source <https://eur-lex.europa.eu/legal-content/EN/TXT/?uri=CELEX%3A02018R0545-20200616#anx_I> .

# 2.3. Extended area of use
eralex:PAVA-AnnexI-2-3 a skos:Concept ;
    skos:inScheme eralex:AnnexIConceptScheme ;
    skos:prefLabel "(I) 2.3. Extended area of use"@en ;
    skos:definition "Extended area of use."@en ;
    skos:broader eralex:PAVA-AnnexI-2 ;
    dcterms:source <https://eur-lex.europa.eu/legal-content/EN/TXT/?uri=CELEX%3A02018R0545-20200616#anx_I> .

# 2.4. Renewed type authorisation
eralex:PAVA-AnnexI-2-4 a skos:Concept ;
    skos:inScheme eralex:AnnexIConceptScheme ;
    skos:prefLabel "(I) 2.4. Renewed type authorisation"@en ;
    skos:definition "Renewed type authorisation."@en ;
    skos:broader eralex:PAVA-AnnexI-2 ;
    dcterms:source <https://eur-lex.europa.eu/legal-content/EN/TXT/?uri=CELEX%3A02018R0545-20200616#anx_I> .

# 2.5. Authorisation in conformity to type
eralex:PAVA-AnnexI-2-5 a skos:Concept ;
    skos:inScheme eralex:AnnexIConceptScheme ;
    skos:prefLabel "(I) 2.5. Authorisation in conformity to type"@en ;
    skos:definition "Authorisation in conformity to type."@en ;
    skos:broader eralex:PAVA-AnnexI-2 ;
    dcterms:source <https://eur-lex.europa.eu/legal-content/EN/TXT/?uri=CELEX%3A02018R0545-20200616#anx_I> .

# 3. Area of use
eralex:PAVA-AnnexI-3 a skos:Concept , sh:NodeShape ;
    skos:inScheme eralex:AnnexIConceptScheme ;
    skos:prefLabel "(I) 3. Area of use"@en ;
    skos:definition "Area of use (Member States, networks, border stations, extended area, whole EU network)."@en ;
    skos:narrower eralex:PAVA-AnnexI-3-1, eralex:PAVA-AnnexI-3-2, eralex:PAVA-AnnexI-3-3, eralex:PAVA-AnnexI-3-4, eralex:PAVA-AnnexI-3-5 ;
    sh:targetClass era:VehicleTypeAuthorisationCase ;
    sh:property [
        sh:path era:areaOfUse ;
        sh:minCount 1 ;
        sh:message "Area of use (era:areaOfUse) must be present for every VehicleTypeAuthorisationCase (Annex I, section 3)."@en ;
        sh:severity sh:Violation
    ] ;
    dcterms:source <https://eur-lex.europa.eu/legal-content/EN/TXT/?uri=CELEX%3A02018R0545-20200616#anx_I> .

# 3.1. Member States
eralex:PAVA-AnnexI-3-1 a skos:Concept ;
    skos:inScheme eralex:AnnexIConceptScheme ;
    skos:prefLabel "(I) 3.1. Member States"@en ;
    skos:definition "Member States."@en ;
    skos:broader eralex:PAVA-AnnexI-3 ;
    dcterms:source <https://eur-lex.europa.eu/legal-content/EN/TXT/?uri=CELEX%3A02018R0545-20200616#anx_I> .

# 3.2. Networks (per Member State)
eralex:PAVA-AnnexI-3-2 a skos:Concept ;
    skos:inScheme eralex:AnnexIConceptScheme ;
    skos:prefLabel "(I) 3.2. Networks (per Member State)"@en ;
    skos:definition "Networks (per Member State)."@en ;
    skos:broader eralex:PAVA-AnnexI-3 ;
    dcterms:source <https://eur-lex.europa.eu/legal-content/EN/TXT/?uri=CELEX%3A02018R0545-20200616#anx_I> .

# 3.3. Border stations
eralex:PAVA-AnnexI-3-3 a skos:Concept ;
    skos:inScheme eralex:AnnexIConceptScheme ;
    skos:prefLabel "(I) 3.3. Border stations"@en ;
    skos:definition "Stations with similar network characteristics in neighbouring Member States when those stations are close to the border."@en ;
    skos:broader eralex:PAVA-AnnexI-3 ;
    dcterms:source <https://eur-lex.europa.eu/legal-content/EN/TXT/?uri=CELEX%3A02018R0545-20200616#anx_I> .

# 3.4. Extended area of use
eralex:PAVA-AnnexI-3-4 a skos:Concept ;
    skos:inScheme eralex:AnnexIConceptScheme ;
    skos:prefLabel "(I) 3.4. Extended area of use"@en ;
    skos:definition "Definition of the extended area of use (only applicable for the authorisation case ‘Extended area of use’)."@en ;
    skos:broader eralex:PAVA-AnnexI-3 ;
    dcterms:source <https://eur-lex.europa.eu/legal-content/EN/TXT/?uri=CELEX%3A02018R0545-20200616#anx_I> .

# 3.5. Whole EU network
eralex:PAVA-AnnexI-3-5 a skos:Concept ;
    skos:inScheme eralex:AnnexIConceptScheme ;
    skos:prefLabel "(I) 3.5. Whole EU network"@en ;
    skos:definition "Whole EU network (applicable for wagons conforming with chapter 7.1.2 of TSI WAG)."@en ;
    skos:broader eralex:PAVA-AnnexI-3 ;
    dcterms:source <https://eur-lex.europa.eu/legal-content/EN/TXT/?uri=CELEX%3A02018R0545-20200616#anx_I> .

# 4. Issuing authority
eralex:PAVA-AnnexI-4 a skos:Concept , sh:NodeShape ;
    skos:inScheme eralex:AnnexIConceptScheme ;
    skos:prefLabel "(I) 4. Issuing authority"@en ;
    skos:definition "Issuing authority (Agency or national safety authority, as applicable)."@en ;
    skos:narrower eralex:PAVA-AnnexI-4-1, eralex:PAVA-AnnexI-4-2 ;
    sh:targetClass era:VehicleTypeAuthorisationCase ;
    sh:property [
        sh:path era:authorisingMemberState ;
        sh:minCount 1 ;
        sh:message "Issuing authority (era:authorisingMemberState) must be present for every VehicleTypeAuthorisationCase (Annex I, section 4)."@en ;
        sh:severity sh:Violation
    ] ;
    sh:or (
        [
            sh:path era:authorisingMemberState ;
            sh:hasValue <http://publications.europa.eu/resource/authority/country/EUR> ;
            sh:message "Annex I 4.1: The Agency is the issuing authority (era:authorisingMemberState = EUR)."@en ;
            sh:severity sh:Info
        ]
        [
            sh:path era:authorisingMemberState ;
            sh:in (
                <http://publications.europa.eu/resource/authority/country/AUT>
                <http://publications.europa.eu/resource/authority/country/BEL>
                <http://publications.europa.eu/resource/authority/country/BGR>
                <http://publications.europa.eu/resource/authority/country/HRV>
                <http://publications.europa.eu/resource/authority/country/CYP>
                <http://publications.europa.eu/resource/authority/country/CZE>
                <http://publications.europa.eu/resource/authority/country/DNK>
                <http://publications.europa.eu/resource/authority/country/EST>
                <http://publications.europa.eu/resource/authority/country/FIN>
                <http://publications.europa.eu/resource/authority/country/FRA>
                <http://publications.europa.eu/resource/authority/country/DEU>
                <http://publications.europa.eu/resource/authority/country/GRC>
                <http://publications.europa.eu/resource/authority/country/HUN>
                <http://publications.europa.eu/resource/authority/country/IRL>
                <http://publications.europa.eu/resource/authority/country/ITA>
                <http://publications.europa.eu/resource/authority/country/LVA>
                <http://publications.europa.eu/resource/authority/country/LTU>
                <http://publications.europa.eu/resource/authority/country/LUX>
                <http://publications.europa.eu/resource/authority/country/MLT>
                <http://publications.europa.eu/resource/authority/country/NLD>
                <http://publications.europa.eu/resource/authority/country/POL>
                <http://publications.europa.eu/resource/authority/country/PRT>
                <http://publications.europa.eu/resource/authority/country/ROU>
                <http://publications.europa.eu/resource/authority/country/SVK>
                <http://publications.europa.eu/resource/authority/country/SVN>
                <http://publications.europa.eu/resource/authority/country/ESP>
                <http://publications.europa.eu/resource/authority/country/SWE>
            ) ;
            sh:message "Annex I 4.2: The national safety authority of the Member State is the issuing authority (era:authorisingMemberState is an EU Member State URI)."@en ;
            sh:severity sh:Info
        ]
    ) ;
    dcterms:source <https://eur-lex.europa.eu/legal-content/EN/TXT/?uri=CELEX%3A02018R0545-20200616#anx_I> .

# 4.1. The Agency
eralex:PAVA-AnnexI-4-1 a skos:Concept ;
    skos:inScheme eralex:AnnexIConceptScheme ;
    skos:prefLabel "(I) 4.1. The Agency"@en ;
    skos:definition "The Agency: area of use covers networks in 1 or more Member States."@en ;
    skos:broader eralex:PAVA-AnnexI-4 ;
    dcterms:source <https://eur-lex.europa.eu/legal-content/EN/TXT/?uri=CELEX%3A02018R0545-20200616#anx_I> .

# 4.2. National safety authority
eralex:PAVA-AnnexI-4-2 a skos:Concept ;
    skos:inScheme eralex:AnnexIConceptScheme ;
    skos:prefLabel "(I) 4.2. National safety authority"@en ;
    skos:definition "The national safety authority of the Member State concerned: area of use covering 1 Member State."@en ;
    skos:broader eralex:PAVA-AnnexI-4 ;
    dcterms:source <https://eur-lex.europa.eu/legal-content/EN/TXT/?uri=CELEX%3A02018R0545-20200616#anx_I> .

# 5. Applicant's information
eralex:PAVA-AnnexI-5 a skos:Concept ;
    skos:inScheme eralex:AnnexIConceptScheme ;
    skos:prefLabel "(I) 5. Applicant's information"@en ;
    skos:definition "Applicant's information (name, address, contact details, VAT, etc.)."@en ;
    dcterms:source <https://eur-lex.europa.eu/legal-content/EN/TXT/?uri=CELEX%3A02018R0545-20200616#anx_I> .

# 6. Contact person information
eralex:PAVA-AnnexI-6 a skos:Concept ;
    skos:inScheme eralex:AnnexIConceptScheme ;
    skos:prefLabel "(I) 6. Contact person information"@en ;
    skos:definition "Contact person information (name, function, address, phone, email, languages)."@en ;
    dcterms:source <https://eur-lex.europa.eu/legal-content/EN/TXT/?uri=CELEX%3A02018R0545-20200616#anx_I> .

# 7. Current vehicle type authorisation holder
eralex:PAVA-AnnexI-7 a skos:Concept ;
    skos:inScheme eralex:AnnexIConceptScheme ;
    skos:prefLabel "(I) 7. Current vehicle type authorisation holder"@en ;
    skos:definition "Current vehicle type authorisation holder (if not first authorisation)."@en ;
    dcterms:source <https://eur-lex.europa.eu/legal-content/EN/TXT/?uri=CELEX%3A02018R0545-20200616#anx_I> .

# 8. Assessment bodies information
eralex:PAVA-AnnexI-8 a skos:Concept ;
    skos:inScheme eralex:AnnexIConceptScheme ;
    skos:prefLabel "(I) 8. Assessment bodies information"@en ;
    skos:definition "Assessment bodies information (notified bodies, designated bodies, CSM RA assessment body)."@en ;
    dcterms:source <https://eur-lex.europa.eu/legal-content/EN/TXT/?uri=CELEX%3A02018R0545-20200616#anx_I> .

# 9. Pre-engagement
eralex:PAVA-AnnexI-9 a skos:Concept ;
    skos:inScheme eralex:AnnexIConceptScheme ;
    skos:prefLabel "(I) 9. Pre-engagement"@en ;
    skos:definition "Pre-engagement (reference to pre-engagement baseline, other project info)."@en ;
    skos:narrower eralex:PAVA-AnnexI-9-1, eralex:PAVA-AnnexI-9-2 ;
    dcterms:source <https://eur-lex.europa.eu/legal-content/EN/TXT/?uri=CELEX%3A02018R0545-20200616#anx_I> .

# 9.1. Reference to pre-engagement baseline
eralex:PAVA-AnnexI-9-1 a skos:Concept ;
    skos:inScheme eralex:AnnexIConceptScheme ;
    skos:prefLabel "(I) 9.1. Reference to pre-engagement baseline"@en ;
    skos:definition "Reference to pre-engagement baseline."@en ;
    skos:broader eralex:PAVA-AnnexI-9 ;
    dcterms:source <https://eur-lex.europa.eu/legal-content/EN/TXT/?uri=CELEX%3A02018R0545-20200616#anx_I> .

# 9.2. Other project information
eralex:PAVA-AnnexI-9-2 a skos:Concept ;
    skos:inScheme eralex:AnnexIConceptScheme ;
    skos:prefLabel "(I) 9.2. Other project information"@en ;
    skos:definition "Other project information relevant to pre-engagement."@en ;
    skos:broader eralex:PAVA-AnnexI-9 ;
    dcterms:source <https://eur-lex.europa.eu/legal-content/EN/TXT/?uri=CELEX%3A02018R0545-20200616#anx_I> .

# 10. Description of the vehicle type
eralex:PAVA-AnnexI-10 a skos:Concept ;
    skos:inScheme eralex:AnnexIConceptScheme ;
    skos:prefLabel "(I) 10. Description of the vehicle type"@en ;
    skos:definition "Description of the vehicle type (type ID, versions, variants, date of record, name, category, subcategory)."@en ;
    skos:narrower eralex:PAVA-AnnexI-10-1, eralex:PAVA-AnnexI-10-2 ;
    dcterms:source <https://eur-lex.europa.eu/legal-content/EN/TXT/?uri=CELEX%3A02018R0545-20200616#anx_I> .

# 10.1. Type identification
eralex:PAVA-AnnexI-10-1 a skos:Concept ;
    skos:inScheme eralex:AnnexIConceptScheme ;
    skos:prefLabel "(I) 10.1. Type identification"@en ;
    skos:definition "Type identification (ID, name, date of record)."@en ;
    skos:broader eralex:PAVA-AnnexI-10 ;
    dcterms:source <https://eur-lex.europa.eu/legal-content/EN/TXT/?uri=CELEX%3A02018R0545-20200616#anx_I> .

# 10.2. Vehicle type versions (when applicable)
eralex:PAVA-AnnexI-10-2 a skos:Concept ;
    skos:inScheme eralex:AnnexIConceptScheme ;
    skos:prefLabel "(I) 10.2. Vehicle type versions (when applicable)"@en ;
    skos:definition "Vehicle type versions as defined in Decision 2011/665/EU Annex II, when applicable."@en ;
    skos:broader eralex:PAVA-AnnexI-10 ;
    dcterms:source <https://eur-lex.europa.eu/legal-content/EN/TXT/?uri=CELEX%3A02018R0545-20200616#anx_I> .

# 10.3. Vehicle type variants (when applicable)
eralex:PAVA-AnnexI-10-3 a skos:Concept ;
    skos:inScheme eralex:AnnexIConceptScheme ;
    skos:prefLabel "(I) 10.3. Vehicle type variants (when applicable)"@en ;
    skos:definition "Vehicle type variants as defined in Decision 2011/665/EU Annex II, when applicable."@en ;
    skos:broader eralex:PAVA-AnnexI-10 ;
    dcterms:source <https://eur-lex.europa.eu/legal-content/EN/TXT/?uri=CELEX%3A02018R0545-20200616#anx_I> .

# 10.4. Date of record in ERATV (not applicable for first authorisation)
eralex:PAVA-AnnexI-10-4 a skos:Concept ;
    skos:inScheme eralex:AnnexIConceptScheme ;
    skos:prefLabel "(I) 10.4. Date of record in ERATV (not applicable for first authorisation)"@en ;
    skos:definition "Date of record in the European Register of Authorised Types of Vehicles (ERATV), not applicable for first authorisation."@en ;
    skos:broader eralex:PAVA-AnnexI-10 ;
    dcterms:source <https://eur-lex.europa.eu/legal-content/EN/TXT/?uri=CELEX%3A02018R0545-20200616#anx_I> .

# 10.5. Type name (*)
eralex:PAVA-AnnexI-10-5 a skos:Concept ;
    skos:inScheme eralex:AnnexIConceptScheme ;
    skos:prefLabel "(I) 10.5. Type name (*)"@en ;
    skos:definition "Type name as specified in Decision 2011/665/EU Annex II."@en ;
    skos:broader eralex:PAVA-AnnexI-10 ;
    dcterms:source <https://eur-lex.europa.eu/legal-content/EN/TXT/?uri=CELEX%3A02018R0545-20200616#anx_I> .

# 10.6. Alternative type name (when applicable)
eralex:PAVA-AnnexI-10-6 a skos:Concept ;
    skos:inScheme eralex:AnnexIConceptScheme ;
    skos:prefLabel "(I) 10.6. Alternative type name (when applicable)"@en ;
    skos:definition "Alternative type name, when applicable, as specified in Decision 2011/665/EU Annex II."@en ;
    skos:broader eralex:PAVA-AnnexI-10 ;
    dcterms:source <https://eur-lex.europa.eu/legal-content/EN/TXT/?uri=CELEX%3A02018R0545-20200616#anx_I> .

# 10.7. Category (*)
eralex:PAVA-AnnexI-10-7 a skos:Concept ;
    skos:inScheme eralex:AnnexIConceptScheme ;
    skos:prefLabel "(I) 10.7. Category (*)"@en ;
    skos:definition "Category of the vehicle type as specified in Decision 2011/665/EU Annex II."@en ;
    skos:broader eralex:PAVA-AnnexI-10 ;
    dcterms:source <https://eur-lex.europa.eu/legal-content/EN/TXT/?uri=CELEX%3A02018R0545-20200616#anx_I> .

# 10.8. Subcategory (*)
eralex:PAVA-AnnexI-10-8 a skos:Concept ;
    skos:inScheme eralex:AnnexIConceptScheme ;
    skos:prefLabel "(I) 10.8. Subcategory (*)"@en ;
    skos:definition "Subcategory of the vehicle type as specified in Decision 2011/665/EU Annex II."@en ;
    skos:broader eralex:PAVA-AnnexI-10 ;
    dcterms:source <https://eur-lex.europa.eu/legal-content/EN/TXT/?uri=CELEX%3A02018R0545-20200616#anx_I> .

# 11. Information on the vehicles
eralex:PAVA-AnnexI-11 a skos:Concept ;
    skos:inScheme eralex:AnnexIConceptScheme ;
    skos:prefLabel "(I) 11. Information on the vehicles"@en ;
    skos:definition "Information on the vehicles (EVN numbers, pre-reserved numbers, other identification)."@en ;
    skos:narrower eralex:PAVA-AnnexI-11-1, eralex:PAVA-AnnexI-11-2 ;
    dcterms:source <https://eur-lex.europa.eu/legal-content/EN/TXT/?uri=CELEX%3A02018R0545-20200616#anx_I> .

# 11.1. EVN numbers
eralex:PAVA-AnnexI-11-1 a skos:Concept ;
    skos:inScheme eralex:AnnexIConceptScheme ;
    skos:prefLabel "(I) 11.1. EVN numbers"@en ;
    skos:definition "European Vehicle Numbers (EVN) assigned to the vehicles."@en ;
    skos:broader eralex:PAVA-AnnexI-11 ;
    dcterms:source <https://eur-lex.europa.eu/legal-content/EN/TXT/?uri=CELEX%3A02018R0545-20200616#anx_I> .

# 11.2. Other identification
eralex:PAVA-AnnexI-11-2 a skos:Concept ;
    skos:inScheme eralex:AnnexIConceptScheme ;
    skos:prefLabel "(I) 11.2. Other identification"@en ;
    skos:definition "Other identification (pre-reserved numbers, etc.)."@en ;
    skos:broader eralex:PAVA-AnnexI-11 ;
    dcterms:source <https://eur-lex.europa.eu/legal-content/EN/TXT/?uri=CELEX%3A02018R0545-20200616#anx_I> .

# 12. Reference to existing vehicle type authorisation (not applicable in case of first authorisation) (M)
eralex:PAVA-AnnexI-12 a skos:Concept ;
    skos:inScheme eralex:AnnexIConceptScheme ;
    skos:prefLabel "(I) 12. Reference to existing vehicle type authorisation (not applicable in case of first authorisation)"@en ;
    skos:definition "Reference to existing vehicle type authorisation, not applicable for first authorisation."@en ;
    skos:related era-va-authcase:RENEW, era-va-authcase:EXT, era-va-authcase:NEW, era-va-authcase:C2T ;
    dcterms:source <https://eur-lex.europa.eu/legal-content/EN/TXT/?uri=CELEX%3A02018R0545-20200616#anx_I> .

# 13. Description of the changes as compared to the authorised vehicle type (only applicable in case of a new authorisation) (M)
eralex:PAVA-AnnexI-13 a skos:Concept ;
    skos:inScheme eralex:AnnexIConceptScheme ;
    skos:prefLabel "(I) 13. Description of the changes as compared to the authorised vehicle type (only applicable in case of a new authorisation)"@en ;
    skos:definition "Description of the changes as compared to the authorised vehicle type (only applicable in case of a new authorisation)."@en ;
    skos:related eralex:PAVA-AnnexI-2-2, era-va-authcase:NEW ;
    dcterms:source <https://eur-lex.europa.eu/legal-content/EN/TXT/?uri=CELEX%3A02018R0545-20200616#anx_I> .

# 16. Applicable rules (M)
eralex:PAVA-AnnexI-16 a skos:Concept ;
    skos:inScheme eralex:AnnexIConceptScheme ;
    skos:prefLabel "(I) 16. Applicable rules (M)"@en ;
    skos:definition "Applicable rules (TSIs, national rules, non-applications, updated rules, etc.)."@en ;
    skos:narrower eralex:PAVA-AnnexI-16-1, eralex:PAVA-AnnexI-16-2, eralex:PAVA-AnnexI-16-3, eralex:PAVA-AnnexI-16-4, eralex:PAVA-AnnexI-16-5, eralex:PAVA-AnnexI-16-6, eralex:PAVA-AnnexI-16-7 ;
    dcterms:source <https://eur-lex.europa.eu/legal-content/EN/TXT/?uri=CELEX%3A02018R0545-20200616#anx_I> .

# 16.1. TSIs
eralex:PAVA-AnnexI-16-1 a skos:Concept ;
    skos:inScheme eralex:AnnexIConceptScheme ;
    skos:prefLabel "(I) 16.1. TSIs"@en ;
    skos:definition "Technical Specifications for Interoperability (TSIs), including the legal reference in the Official Journal of the European Union."@en ;
    skos:broader eralex:PAVA-AnnexI-16 ;
    dcterms:source <https://eur-lex.europa.eu/legal-content/EN/TXT/?uri=CELEX%3A02018R0545-20200616#anx_I> .

# 16.2. Specific TSIs clauses for an area of use covering the whole EU network (when applicable)
eralex:PAVA-AnnexI-16-2 a skos:Concept ;
    skos:inScheme eralex:AnnexIConceptScheme ;
    skos:prefLabel "(I) 16.2. Specific TSIs clauses for an area of use covering the whole EU network (when applicable)"@en ;
    skos:definition "Specific TSIs clauses for an area of use covering the whole EU network, when applicable."@en ;
    skos:broader eralex:PAVA-AnnexI-16 ;
    dcterms:source <https://eur-lex.europa.eu/legal-content/EN/TXT/?uri=CELEX%3A02018R0545-20200616#anx_I> .

# 16.3. Specification of the selection of requirements from a newer version of a TSI as compared to the TSI applicable for the assessment (including withdrawn requirements) (when applicable)
eralex:PAVA-AnnexI-16-3 a skos:Concept ;
    skos:inScheme eralex:AnnexIConceptScheme ;
    skos:prefLabel "(I) 16.3. Specification of the selection of requirements from a newer version of a TSI as compared to the TSI applicable for the assessment (including withdrawn requirements) (when applicable)"@en ;
    skos:definition "Specification of the selection of requirements from a newer version of a TSI as compared to the TSI applicable for the assessment, including withdrawn requirements, when applicable."@en ;
    skos:broader eralex:PAVA-AnnexI-16 ;
    dcterms:source <https://eur-lex.europa.eu/legal-content/EN/TXT/?uri=CELEX%3A02018R0545-20200616#anx_I> .

# 16.4. National rules (when applicable)
eralex:PAVA-AnnexI-16-4 a skos:Concept ;
    skos:inScheme eralex:AnnexIConceptScheme ;
    skos:prefLabel "(I) 16.4. National rules (when applicable)"@en ;
    skos:definition "National rules, when applicable."@en ;
    skos:broader eralex:PAVA-AnnexI-16 ;
    dcterms:source <https://eur-lex.europa.eu/legal-content/EN/TXT/?uri=CELEX%3A02018R0545-20200616#anx_I> .

# 16.5. Non-applications of TSIs according to the provisions of Article 7 of Directive (EU) 2016/797 (when applicable)
eralex:PAVA-AnnexI-16-5 a skos:Concept ;
    skos:inScheme eralex:AnnexIConceptScheme ;
    skos:prefLabel "(I) 16.5. Non-applications of TSIs according to the provisions of Article 7 of Directive (EU) 2016/797 (when applicable)"@en ;
    skos:definition "Non-applications of TSIs according to the provisions of Article 7 of Directive (EU) 2016/797, when applicable."@en ;
    skos:broader eralex:PAVA-AnnexI-16 ;
    dcterms:source <https://eur-lex.europa.eu/legal-content/EN/TXT/?uri=CELEX%3A02018R0545-20200616#anx_I> .

# 16.6. Applicable rules for the extended area of use
eralex:PAVA-AnnexI-16-6 a skos:Concept ;
    skos:inScheme eralex:AnnexIConceptScheme ;
    skos:prefLabel "(I) 16.6. Applicable rules for the extended area of use"@en ;
    skos:definition "Applicable rules for the extended area of use."@en ;
    skos:broader eralex:PAVA-AnnexI-16 ;
    dcterms:source <https://eur-lex.europa.eu/legal-content/EN/TXT/?uri=CELEX%3A02018R0545-20200616#anx_I> .

# 16.7. Updated TSIs and/or national rules (only applicable for renewed type authorisation)
eralex:PAVA-AnnexI-16-7 a skos:Concept ;
    skos:inScheme eralex:AnnexIConceptScheme ;
    skos:prefLabel "(I) 16.7. Updated TSIs and/or national rules (only applicable for renewed type authorisation)"@en ;
    skos:definition "Updated TSIs and/or national rules, only applicable for renewed type authorisation."@en ;
    skos:broader eralex:PAVA-AnnexI-16 ;
    dcterms:source <https://eur-lex.europa.eu/legal-content/EN/TXT/?uri=CELEX%3A02018R0545-20200616#anx_I> .

# 17. Applicant's confirmation and signature
eralex:PAVA-AnnexI-17 a skos:Concept ;
    skos:inScheme eralex:AnnexIConceptScheme ;
    skos:prefLabel "(I) 17. Applicant's confirmation and signature"@en ;
    skos:definition "Applicant's confirmation and signature."@en ;
    dcterms:source <https://eur-lex.europa.eu/legal-content/EN/TXT/?uri=CELEX%3A02018R0545-20200616#anx_I> .

# 18. Annexes
eralex:PAVA-AnnexI-18 a skos:Concept ;
    skos:inScheme eralex:AnnexIConceptScheme ;
    skos:prefLabel "(I) 18. Annexes"@en ;
    skos:definition "Annexes (supporting evidence, mapping tables, declarations, technical files, etc.)."@en ;
    dcterms:source <https://eur-lex.europa.eu/legal-content/EN/TXT/?uri=CELEX%3A02018R0545-20200616#anx_I> .
