


#################################################################
#
#    Concept Schemes
#
#################################################################



erava-orgroletasks:OrganisationRoleTasks a skos:ConceptScheme ; 
    dct:issued "2024-12-06"^^xsd:date ;
    # dct:modified "_RESERVED_"^^xsd:date ;
    cc:license <https://creativecommons.org/licenses/by/4.0/> ;
    rdfs:label "Organisations - task groups to be executed by Agents, within Organisations having a certain era:Role"@en ;
    rdfs:comment """This SKOS Concept Scheme is used to define what `org:Role`s are executed by Agents belonging to a certain Organisation.

Organisations play certain roles (`era:hasRole`), which are realised by the execution of tasks by Agents working within them. In the W3C Organisation ontology,
these tasks are grouped under `org:Role`, a subClassof skos:Concept.

This Concept scheme provides the task groups which exist in each of the organisation roles ERA is executing processes with."""@en ;
    skos:example """To be provided"""@en ;
    rdfs:seeAlso "era-skos/era-skos-OrgRoles.ttl" ;
    dct:source <http://data.europa.eu/949/concepts/organisation-roles/OrgRoles> ;
    skos:prefLabel "Tasks executed by Agents belonging to a certain Organisation"@en ;
    skos:editorialNote ""@en ;
    dct:title "Concept scheme grouping tasks belonging to organisation roles"@en .



#################################################################
#
#    Concept instances
#
#################################################################

    


########## Tasks executed by Agents belonging to a certain Organisation ##########

#### MANUFACTURER

erava-orgroletasks:va-applicant a org:Role ; # skos:Concept
    skos:inScheme erava-orgroletasks:OrganisationRoleTasks ;
    dct:source <http://data.europa.eu/eli/reg_impl/2018/545/2020-06-16#art_3> ;
    skos:notation "The agent executing the role of applicant of a vehicle (type) authorisation process."@en ;
    skos:prefLabel "Responsable agent, representing the applicant for vehicle authorisation" ;
    skos:definition "See Article 3 of the legal reference."@en .    

erava-orgroletasks:ic-applicant a org:Role ; # skos:Concept
    skos:inScheme erava-orgroletasks:OrganisationRoleTasks ;
    dct:source <https://eur-lex.europa.eu/legal-content/EN/TXT/?uri=CELEX%3A02016L0797-20200528#art_10> ;
    skos:notation "The agent executing the role of applicant of a process to bring an IC to the market."@en ;
    skos:prefLabel "Responsable agent, representing the applicant for placing an IC on the market" ;
    skos:definition """In order to establish the ‘EC’ declaration of conformity or suitability for use of an interoperability constituent, the manufacturer or his authorised
 representative shall apply the provisions laid down by the relevant TSIs."""@en .    

erava-orgroletasks:ss-applicant a org:Role ; # skos:Concept
    skos:inScheme erava-orgroletasks:OrganisationRoleTasks ;
    dct:source <https://eur-lex.europa.eu/legal-content/EN/TXT/?uri=CELEX%3A02016L0797-20200528#art_15> ;
    skos:notation "The agent executing the role of applicant of a process to bring a Subsystem to the market."@en ;
    skos:prefLabel "Responsable agent, representing the applicant for placing a Subsystem on the market" ;
    skos:definition """The applicant shall establish the ‘EC’ declaration of verification of a subsystem. The applicant shall declare on his sole responsibility that 
the subsystem concerned has been subject to the relevant verification procedures and that it satisfies the requirements of relevant Union law and any relevant national rule."""@en .

#### AUTHORISING ENTITY

## Vehicle Authorisation

erava-orgroletasks:va-projectmanager a org:Role ; # skos:Concept
    skos:inScheme erava-orgroletasks:OrganisationRoleTasks ;
    dct:source <http://data.europa.eu/eli/reg_impl/2018/545/2020-06-16#art_4> ;
    skos:notation "The agent executing the role of project manager at the authorising entity executing a vehicle authorisation process."@en ;
    rdfs:comment "Not all authorising entities have agents executing this role separately."@en ;
    skos:prefLabel "Agent, representing authorising entity for vehicle authorisation, managing the project of a vehicle (type) authorisation." ;
    skos:definition "See Article 4 of the legal reference."@en .    

erava-orgroletasks:va-assessor a org:Role ; # skos:Concept
    skos:inScheme erava-orgroletasks:OrganisationRoleTasks ;
    dct:source <http://data.europa.eu/eli/reg_impl/2018/545/2020-06-16#art_4> ;
    skos:notation "The agent executing the role of assessor at the authorising entity executing a vehicle authorisation process."@en ;
    skos:prefLabel "Agent, representing authorising entity for vehicle authorisation, executing the analysis and assessment tasks of a vehicle (type) authorisation." ;
    skos:definition "See Article 4 of the legal reference."@en .    

erava-orgroletasks:va-qualitymanager a org:Role ; # skos:Concept
    skos:inScheme erava-orgroletasks:OrganisationRoleTasks ;
    dct:source <http://data.europa.eu/eli/reg_impl/2018/545/2020-06-16#art_4> ;
    skos:notation "The agent executing the role of quality manager at the authorising entity executing a vehicle authorisation process."@en ;
    rdfs:comment "Not all authorising entities have agents executing this role separately."@en ;
    skos:prefLabel "Agent, representing authorising entity for vehicle authorisation, and responsible for the quality assurance" ;
    skos:definition "See Article 4 of the legal reference."@en .    

erava-orgroletasks:va-decisionmaker a org:Role ; # skos:Concept
    skos:inScheme erava-orgroletasks:OrganisationRoleTasks ;
    dct:source <http://data.europa.eu/eli/reg_impl/2018/545/2020-06-16#art_4> ;
    skos:notation "The agent deciding at the authorising entity to finalise a vehicle authorisation process."@en ;
    skos:prefLabel "Agent, representing authorising entity for vehicle authorisation, and responsible for the final authorisation" ;
    skos:definition "See Article 4 of the legal reference."@en .    

#### Assessment Body (NoBo, DeBo, AsBo, ISA, etc...)

erava-orgroletasks:ab-assessor a org:Role ; # skos:Concept
    skos:inScheme erava-orgroletasks:OrganisationRoleTasks ;
    dct:source <> ;
    skos:notation "The agent executing the role of assessor at the accredited body executing a certification process."@en ;
    skos:prefLabel "Agent, representing an assessment body, and responsible for the assessment (any reference chapter)" ;
    skos:definition ""@en . 

erava-orgroletasks:ab-qualitymanager a org:Role ; # skos:Concept
    skos:inScheme erava-orgroletasks:OrganisationRoleTasks ;
    dct:source <> ;
    skos:notation "The agent executing the role of quality manager at the accredited body executing a certification process."@en ;
    skos:prefLabel "Agent, representing an assessment body, and responsible for the quality assurance" ;
    skos:definition ""@en .  

erava-orgroletasks:ab-decisionmaker a org:Role ; # skos:Concept
    skos:inScheme erava-orgroletasks:OrganisationRoleTasks ;
    dct:source <> ;
    skos:notation "The agent executing the role of decision maker at the accredited body signing the final result of a certification process."@en ;
    skos:prefLabel "Agent, representing an assessment body, and responsible for the final certification process result." ;
    skos:definition ""@en .  

erava-orgroletasks:int-assessor a org:Role ; # skos:Concept
    skos:inScheme erava-orgroletasks:OrganisationRoleTasks ;
    dct:source <https://eur-lex.europa.eu/legal-content/EN/TXT/?uri=CELEX%3A02016L0797-20200528#art_35> ;
    skos:notation "The agent executing the role of assessor at the accredited in-house body executing a certification process."@en ;
    skos:prefLabel "Agent, representing an accredited in-house body, and responsible for the assessment (any reference chapter)" ;
    skos:definition ""@en . 

erava-orgroletasks:int-qualitymanager a org:Role ; # skos:Concept
    skos:inScheme erava-orgroletasks:OrganisationRoleTasks ;
    dct:source <https://eur-lex.europa.eu/legal-content/EN/TXT/?uri=CELEX%3A02016L0797-20200528#art_35> ;
    skos:notation "The agent executing the role of quality manager at the accredited in-house body executing a certification process."@en ;
    skos:prefLabel "Agent, representing an accredited in-house body, and responsible for the quality assurance" ;
    skos:definition ""@en .  

erava-orgroletasks:int-decisionmaker a org:Role ; # skos:Concept
    skos:inScheme erava-orgroletasks:OrganisationRoleTasks ;
    dct:source <https://eur-lex.europa.eu/legal-content/EN/TXT/?uri=CELEX%3A02016L0797-20200528#art_35> ;
    skos:notation "The agent executing the role of decision maker at the accredited in-house body signing the final result of a certification process."@en ;
    skos:prefLabel "Agent, representing an accredited in-house body, and responsible for the final certification process result." ;
    skos:definition ""@en .  

#### ISS - to be provided. A link is to be made with the authorisations needed to execute certain tasks.